progress

HOL_To_IMP/Refinements/HOL_TCN_To_IMP_Temp.thy
@@ -1,5 +1,5 @@
 theory HOL_TCN_To_IMP_Temp
-  imports HOL_To_IMP_Primitives "IMP.HOL_TCN_To_IMP" (* HOL_Nat_To_IMP.Compile_HOL_Nat_To_IMP *)
+  imports HOL_Nat_To_IMP.IMP_Terminates_With "IMP.HOL_TCN_To_IMP" (* HOL_Nat_To_IMP.Compile_HOL_Nat_To_IMP *)
 (* TODO: rearrange import of stuff from Compile *)
 begin
 
@@ -11,7 +11,7 @@ method repeat methods m = (m; repeat \<open>m\<close>)?
 (* definition "interp_time1 frgt g vs_arg_g = T_f_from_reg frgt g vs_arg_g" *)
 (* definition "interp_time frgt = sum_map (\<lambda>(g, vs_arg_g). interp_time1 frgt g vs_arg_g)" *)
   (* assumes "f_imp = to_imp_tc_1 f_args crgt r0 f" *)
-  (* assumes "set (special_regs f_args crgt r t) \<subseteq> set stale" *)
+  (* assumes "set (special_regs f_args crgt r t) \<subseteq> set keep" *)
 
 abbreviation "lookups names (s :: state) \<equiv> map s names"
 
@@ -33,35 +33,143 @@ definition "tinterp_time frgt crgt =
 abbreviation "lookups names (s :: state) \<equiv> map s names"
 abbreviation "lookup_args crgt g \<equiv> lookups (args_from_crgt crgt g)"
 
-(* definition "is_call_in t f = (f \<in> set (calls t))" *)
+(* note: lookups xs s = map s xs *)
+lemma map_eq_on_subset_eq: fixes A assumes "set xs \<subseteq> A" "f = g on A" shows "map f xs = map g xs"
+  using assms unfolding eq_on_def by (induction xs) auto
 
-(* the term is tail-recursive, "special" registers are marked stale,
-   and the argument list of f and of any called functions is distinct *)
-definition "compiler_args_invar f_args crgt bs stale t \<longleftrightarrow>
+abbreviation disjoint :: "'a set \<Rightarrow> 'a set \<Rightarrow> bool"  (infix \<open>\<inter>\<^sub>\<emptyset>\<close> 60)
+  where "A \<inter>\<^sub>\<emptyset> B \<equiv> A \<inter> B = {}" for A B
+
+lemma disjoint_subset2:
+  fixes A B
+  assumes "B \<subseteq> B'"
+  assumes "A \<inter>\<^sub>\<emptyset> B'"
+  shows "A \<inter>\<^sub>\<emptyset> B"
+  using assms by blast
+
+definition "compiler_args_invar crgt f_args bs keep t \<longleftrightarrow>
   HOL_TCN_Timing.invar t
-  \<and> set (reserved_regs f_args crgt bs t) \<subseteq> set stale
   \<and> distinct f_args
-  \<and> (\<forall>(g,_) \<in> set (calls t). distinct (args_from_crgt crgt g))
-  \<and> (\<forall>(g,ts) \<in> set (calls t). length ts = length (args_from_crgt crgt g))"
+  \<and> set f_args \<inter>\<^sub>\<emptyset> set (call_registers crgt t)
+  \<and> set bs \<inter>\<^sub>\<emptyset> set (call_registers crgt t)
+  \<and> set bs \<inter>\<^sub>\<emptyset> set f_args
+  \<and> set keep \<inter>\<^sub>\<emptyset> set f_args
+  \<and> set keep \<inter>\<^sub>\<emptyset> set (call_registers crgt t)
+  \<and> (\<forall>g\<in>fst ` set (calls t). distinct (args_from_crgt crgt g))
+  \<and> (\<forall>(g,ts)\<in>set (calls t). length ts = length (args_from_crgt crgt g))"
+(*
+- The term must be tail-recursive, i.e. satisfy the invariant.
+
+- Register lists that are written to must be distinct, otherwise writing a later register will
+  overwrite a register earlier in the list. Thus, f_args and g_args for each called g must be
+  distinct: f_args is written before a tail call, g_args on a call to g.
+
+- If a value is stored to a register (list) R, then later the register (list) W is written to, and
+  then later that value should be read back from R, R and W must be disjoint.
+  Otherwise, the write to W could overwrite the value in R. We consider "f_args" and "bs" to be
+  stored at the beginning of execution, and "keep" and "r" to be read after execution. We have:
+
+  - f_args: stored at the beginning of execution, written while preparing for a tail call, read at argument variable read
+  - bs: stored at the beginning of execution, read at bound variable read
+  - g_args for each call of a function g: written and then immediately read by the called function.
+  - g_ret for each call of a function g: written after the call and the immediately read for copying.
+  - r: written immediately before the end of execution, read after execution
+  - keep: stored before execution, read after execution.
+
+  Conflict matrix:
+
+         W: f_args bs g_args g_ret r
+    R:     +------------------------
+    f_args |        -      X     X -
+    bs     |     X         X     X -
+    g_args |     -  -      -     - -
+    g_ret  |     -  -      -     - -
+    r      |     -  -      -     - -
+    keep   |     X  -      X     X X
+
+  We special-case the keep/r conflict: instead of requiring keep and r to be disjoint, the
+  correctness theorems show that "keep" except "r" is preserved.
+
+- At each call site, the correct number of arguments must be provided to the called function.
+*)
+
+lemma compiler_args_invar_subset:
+  assumes "invar t"
+  assumes "set (calls t) \<subseteq> set (calls t')"
+  assumes "compiler_args_invar crgt f_args bs keep t'"
+  shows "compiler_args_invar crgt f_args bs keep t"
+  using disjoint_subset2[where B = "set (call_registers crgt t)" and B' = "set (call_registers crgt t')"]
+  using assms call_registers_set unfolding compiler_args_invar_def split_beta by auto
+
+
+(* 
+  \<and> (\<forall>(g, _) \<in> set (calls t).
+      distinct (args_from_crgt crgt g)
+      \<and> set f_args \<inter> set (args_from_crgt crgt g) = {}
+      \<and> ret_from_crgt crgt g \<notin> set f_args
+      \<and> set bs \<inter> set (args_from_crgt crgt g) = {}
+      \<and> ret_from_crgt crgt g \<notin> set bs) *)
+
+(*
+lemma compiler_args_invar_hCall:
+  assumes "invar (hCall gr ts)"
+  assumes "compiler_args_invar crgt f_args (hCall gr ts)"
+  assumes "t \<in> set ts"
+  shows "compiler_args_invar crgt f_args t"
+  using assms unfolding compiler_args_invar_def by simp
+
+lemma compiler_args_invar_hTAIL:
+  assumes "invar (hTAIL ts)"
+  assumes "compiler_args_invar f_args crgt bs keep (hTAIL ts)"
+  assumes "t \<in> set ts"
+  shows "compiler_args_invar f_args crgt bs keep t"
+proof-
+  let ?t = "hTAIL ts"
+  have calls_subset: "set (calls t) \<subseteq> set (calls ?t)" using assms by auto
+  show "compiler_args_invar f_args crgt bs keep t"
+  unfolding compiler_args_invar_def proof (repeat \<open>rule conjI\<close>)
+    show "HOL_TCN_Timing.invar t" using no_tails_invar assms by simp
+  next
+    have "set (reserved_regs f_args crgt bs t) \<subseteq> set (reserved_regs f_args crgt bs ?t)"
+      unfolding reserved_regs_def using calls_subset assms by auto
+    then show "set (reserved_regs f_args crgt bs t) \<subseteq> set keep"
+      using assms unfolding compiler_args_invar_def by auto
+  next
+    show "distinct f_args" using assms unfolding compiler_args_invar_def by simp
+  next
+    show "\<forall>(g,_)\<in>set (calls t). distinct (args_from_crgt crgt g)"
+      using assms calls_subset unfolding compiler_args_invar_def split_beta by blast
+  next
+    show "\<forall>(g, ts)\<in>set (calls t). length ts = length (args_from_crgt crgt g)"
+      using assms calls_subset unfolding compiler_args_invar_def split_beta by blast
+  qed
+qed*)
+
+(*
+fun subterms1 where
+  "subterms1 (hLet t1 t2) = [t1, t2]" |
+  "subterms1 (hIf t1 t2 t3) = [t1, t2, t3]" |
+  "subterms1 (hCall _ ts) = ts" |
+  "subterms1 (hTAIL ts) = ts" |
+  "subterms1 _ = []"*)
+
+
 
 (* the "state" of the HOL-TCN execution (args, bounds) is related
    to the state of the IMP-TC execution *)
 definition "relate_exec_state f_args bs vs_arg vs_b s \<longleftrightarrow>
   lookups f_args s = vs_arg \<and> lookups bs s = vs_b"
 
+(*
 definition "called_correctness crgt frgt fs \<longleftrightarrow> (\<forall>f \<in> fs.
     HOL_Nat_To_IMP.terminates_with_res_time_order_IMP
       (com_from_crgt crgt f) (ret_from_crgt crgt f)
       (f_from_frgt frgt f o lookup_args crgt f) (T_f_from_frgt frgt f o lookup_args crgt f))" (* can we replace ...  with existential ? *)
+*)
 
 definition "relate_rgt_correctness frgt crgt fs \<longleftrightarrow> (\<forall>f \<in> fs.
-  \<forall>s. terminates_with_res_IMP (com_from_crgt crgt f) s (ret_from_crgt crgt f)
-        (f_from_frgt frgt f (lookup_args crgt f s)))"
+  \<forall>s. terminates_with_res_IMP (com_from_crgt crgt f) s (ret_from_crgt crgt f) (f_from_frgt frgt f (lookup_args crgt f s)))"
 
-
-(* note: lookups xs s = map s xs *)
-lemma map_eq_on_subset_eq: fixes A assumes "set xs \<subseteq> A" "f = g on A" shows "map f xs = map g xs"
-  using assms unfolding eq_on_def by (induction xs) auto
 
 lemma snoc_obtain:
   assumes "xs \<noteq> []"
@@ -130,37 +238,41 @@ lemma mapi_ix2:
   using assms nth_append by metis *)
 
 lemma nth_append_length_eq:
-  assumes "length xs = length ys"
-  shows "(xs @ y # zs) ! (length ys) = y"
+  assumes "length xs = n"
+  shows "(xs @ y # zs) ! n = y"
   apply (subst nth_append) using assms by simp
 
 lemma copy_list_sem:
   assumes "length xs = length ys"
-  assumes "distinct (xs @ ys)" (* technically, this assumption could be weakened *)
+  assumes "distinct ys"
+  assumes "set xs \<inter> set ys = {}"
+    (* technically, these assumptions could be weakened *)
   obtains s' where
-    "f \<turnstile> (t_seqs' (map (\<lambda>i. (ys ! i) ::= A (V (xs ! i))) [0..<length xs]),s) \<Rightarrow>\<^bsup>Suc (2 * length xs)\<^esup> s'"
-    "lookups xs s = lookups ys s'" "s = s' on (- set ys)"
+    "f \<turnstile> (t_seqs' (generate (\<lambda>i. (ys ! i) ::= A (V (xs ! i))) (length xs)),s) \<Rightarrow>\<^bsup>Suc (2 * length xs)\<^esup> s'"
+    "lookups ys s' = lookups xs s" "s' = s on (- set ys)"
 using assms proof (induction xs ys arbitrary: thesis rule: snoc_list_induct2)
   case Nil
-  then show ?case using tSkip_tE by auto
+  then show ?case unfolding generate_def using tSkip_tE by auto
 next
   case (snoc xs x ys y)
 
-  let ?cs = "\<lambda>xs ys. map (\<lambda>i. (ys ! i) ::= A (V (xs ! i)) :: tcom) [0..<length xs]"
+  let ?cs = "\<lambda>xs ys. generate (\<lambda>i. (ys ! i) ::= A (V (xs ! i)) :: tcom) (length xs)"
 
   let ?cs1 = "?cs xs ys"
   let ?c2 = "y ::= A (V x) :: tcom"
   let ?cs' = "?cs (xs @ [x]) (ys @ [y])"
 
-  have cs': "?cs' = ?cs1 @ [?c2]" by (simp add: snoc nth_append_left nth_append_length_eq)
+  have cs': "?cs' = ?cs1 @ [?c2]"
+    apply (simp add: generate_snoc)
+    unfolding generate_def using nth_append_left snoc by fastforce
 
   from snoc obtain s2 where ih:
       "f \<turnstile> (t_seqs' ?cs1, s) \<Rightarrow>\<^bsup>Suc (2 * length xs)\<^esup> s2"
-      "lookups xs s = lookups ys s2" "s = s2 on (- set ys)"
+      "lookups ys s2 = lookups xs s" "s2 = s on (- set ys)"
     by auto
   moreover obtain s3 where step:
       "f \<turnstile> (?c2, s2) \<Rightarrow>\<^bsup>Suc (Suc 0)\<^esup> s3"
-      "s3 y = s2 x" "s2 = s3 on (- {y})"
+      "s3 y = s2 x" "s3 = s2 on (- {y})"
     by fastforce
   ultimately have "f \<turnstile> (t_seqs' ?cs1;; ?c2, s) \<Rightarrow>\<^bsup>Suc (2 * length (xs @ [x]))\<^esup> s3" by auto
   then have "f \<turnstile> (t_seqs' (?cs1 @ [?c2]), s) \<Rightarrow>\<^bsup>Suc (2 * length (xs @ [x]))\<^esup> s3" 
@@ -168,82 +280,106 @@ next
   then have 1: "f \<turnstile> (t_seqs' ?cs', s) \<Rightarrow>\<^bsup>Suc (2 * length (xs @ [x]))\<^esup> s3"
     by (subst cs') assumption
 
-  have 2: "lookups (xs @ [x]) s = lookups (ys @ [y]) s3"
+  have 2: "lookups (ys @ [y]) s3 = lookups (xs @ [x]) s"
     using ih step snoc by auto
 
-  have 3: "s = s3 on (- set (ys @ [y]))"
+  have 3: "s3 = s on (- set (ys @ [y]))"
     using ih step by auto
 
   from 1 2 3 snoc show ?case by blast
 qed (simp add: assms)
 
+lemma copy_list_sem':
+  assumes "length xs = n"
+  assumes "length ys = n"
+  assumes "distinct ys"
+  assumes "set xs \<inter> set ys = {}"
+  obtains s' where
+    "f \<turnstile> (t_seqs' (generate (\<lambda>i. (ys ! i) ::= A (V (xs ! i))) n),s) \<Rightarrow>\<^bsup>Suc (2 * n)\<^esup> s'"
+    "lookups ys s' = lookups xs s" "s' = s on (- set ys)"
+  using copy_list_sem[where xs = xs and ys = ys] assms by auto
 
-
+(*
 lemma cc_call_helper:
   "f \<turnstile> (t_seqs' cs1;; t_seqs' cs2;; c, s) \<Rightarrow>\<^bsup>Suc (Suc z)\<^esup> t \<longleftrightarrow> f \<turnstile> (t_seqs (cs1 @ cs2) c, s) \<Rightarrow>\<^bsup>z\<^esup> t"
-  using tbig_step_t_t_seqs_rewrite by simp
+  using tbig_step_t_t_seqs_rewrite by simp *)
 
 abbreviation "calls_r t \<equiv> set (map fst (calls t))"
+
+lemma Un_Diff_cancel1: "A \<union> B - A = B - A" for A B :: "'a set"
+  by blast
 
 lemma compiler_correct_nt:
   assumes "\<not> tails t"
   assumes "(f,frgt) \<turnstile> (t,vs_b,vs_arg) \<Rightarrow>\<^bsup>z\<^esup> v"
-  assumes "compiler_args_invar f_args crgt bs stale t"
+  assumes "compiler_args_invar crgt f_args bs keep t"
   assumes "relate_rgt_correctness frgt crgt (calls_r t)"
   assumes "relate_exec_state f_args bs vs_arg vs_b s"
   shows "\<exists>z_c s'.
-    f_c \<turnstile> (to_imp_tc f_args crgt bs r stale t,s) \<Rightarrow>\<^bsup>z_c\<^esup> s'
+    f_c \<turnstile> (to_imp_tc f_args crgt bs r keep t,s) \<Rightarrow>\<^bsup>z_c\<^esup> s'
     \<and> s' r = v
-    \<and> s = s' on set stale - {r}"
-using assms proof (induction t arbitrary: vs_b z v bs stale s r crgt)
+    \<and> s' = s on set f_args \<union> set bs \<union> set keep - {r}"
+using assms proof (induction t arbitrary: vs_b z v bs keep s r crgt)
   case (hLet t1 t2)
 
-  let ?r1 = "fresh' stale ''Let.x''"
+  let ?r1 = "fresh' (stale_registers f_args crgt bs keep LET t1 IN t2) ''Let.x''"
+  let ?t1_c = "to_imp_tc f_args crgt bs ?r1 keep t1"
+  let ?t2_c = "to_imp_tc f_args crgt (?r1 # bs) r (?r1 # keep) t2"
 
   have no_tails: "\<not> HOL_TCN_Timing.tails t1" "\<not> HOL_TCN_Timing.tails t2" using hLet by simp_all
 
-  obtain z1 v1 z2 where inv: "z = z1 + z2" "(f, frgt) \<turnstile> (t1, vs_b, vs_arg) \<Rightarrow>\<^bsup>z1\<^esup>  v1" "(f, frgt) \<turnstile> (t2, v1 # vs_b, vs_arg) \<Rightarrow>\<^bsup>z2\<^esup>  v"
+  obtain z1 v1 z2 where
+      "z = z1 + z2" and inv: "(f, frgt) \<turnstile> (t1, vs_b, vs_arg) \<Rightarrow>\<^bsup>z1\<^esup> v1" "(f, frgt) \<turnstile> (t2, v1 # vs_b, vs_arg) \<Rightarrow>\<^bsup>z2\<^esup> v"
     using hLet_case hLet.prems by blast
 
-  have args_invar: "compiler_args_invar f_args crgt bs stale t1" "compiler_args_invar f_args crgt (?r1 # bs) (?r1 # stale) t2"
-    using hLet unfolding compiler_args_invar_def reserved_regs_def split_beta by auto
+  have args_invar1: "compiler_args_invar crgt f_args bs keep t1"
+    using hLet.prems compiler_args_invar_subset[where t' = "LET t1 IN t2"] by simp
+
+  have "?r1 \<notin> set f_args"
+    apply (rule contra_subsetD[OF _ fresh_not_in_stale])
+    unfolding stale_registers_def by simp
+  moreover have "?r1 \<notin> set (call_registers crgt t2)"
+    apply (rule contra_subsetD[OF _ fresh_not_in_stale])
+    using call_registers_set unfolding stale_registers_def by auto
+  moreover have "compiler_args_invar crgt f_args bs keep t2"
+    using hLet.prems compiler_args_invar_subset[where t' = "LET t1 IN t2"] by simp
+  ultimately have args_invar2: "compiler_args_invar crgt f_args (?r1 # bs) (?r1 # keep) t2"
+    using hLet.prems(3) unfolding compiler_args_invar_def by auto
 
   have rel_rgt: "relate_rgt_correctness frgt crgt (calls_r t1)" "relate_rgt_correctness frgt crgt (calls_r t2)"
-    using hLet unfolding relate_rgt_correctness_def by auto
+    using hLet unfolding relate_rgt_correctness_def by simp_all
 
   have rel_state1: "relate_exec_state f_args bs vs_arg vs_b s" using hLet by blast
 
-  obtain z1_c s2 where
-    ih1: "f_c \<turnstile> (to_imp_tc f_args crgt bs ?r1 stale t1, s) \<Rightarrow>\<^bsup>z1_c\<^esup>  s2" "s2 ?r1 = v1" "s = s2 on set stale - {?r1}"
-    using no_tails inv args_invar rel_rgt rel_state1 hLet by metis
+  obtain z1_c s2 where ih1:
+      "f_c \<turnstile> (?t1_c, s) \<Rightarrow>\<^bsup>z1_c\<^esup> s2" "s2 ?r1 = v1" "s2 = s on set f_args \<union> set bs \<union> set keep - {?r1}"
+    using hLet.IH(1) no_tails(1) inv(1) args_invar1 rel_rgt(1) rel_state1 by blast
 
-  have res_reg_subset: "set f_args \<subseteq> set stale - {?r1}" "set bs \<subseteq> set stale - {?r1}"
-    using hLet.prems(3) fresh_not_in_stale unfolding compiler_args_invar_def reserved_regs_def by simp_all
+  have s_like_s2: "s2 = s on set f_args \<union> set bs \<union> set keep" (* TODO *)
+    by (smt (verit) DiffI Un_iff eq_on_def fresh_not_in_stale ih1(3) set_append singletonD stale_registers_def)
+  then have rel_state2: "relate_exec_state f_args (?r1 # bs) vs_arg (v1 # vs_b) s2"
+    using hLet.prems(5) unfolding relate_exec_state_def using ih1 by fastforce
 
-  have rel_state2: "relate_exec_state f_args (?r1 # bs) vs_arg (v1 # vs_b) s2"
-    using hLet ih1 unfolding relate_exec_state_def apply simp
-    unfolding map_eq_on_subset_eq[OF res_reg_subset(1)] map_eq_on_subset_eq[OF res_reg_subset(2)] by blast
+  obtain z2_c s3 where ih2:
+      "f_c \<turnstile> (?t2_c, s2) \<Rightarrow>\<^bsup>z2_c\<^esup>  s3" "s3 r = v"
+      "s3 = s2 on set f_args \<union> set (?r1 # bs) \<union> set (?r1 # keep) - {r}"
+    using hLet.IH(2) no_tails(2) inv(2) args_invar2 rel_rgt(2) rel_state2 by blast
 
-  obtain z2_c s3 where
-    ih2: "f_c \<turnstile> (to_imp_tc f_args crgt (?r1 # bs) r (?r1 # stale) t2, s2) \<Rightarrow>\<^bsup>z2_c\<^esup>  s3" "s3 r = v" "s2 = s3 on set (?r1 # stale) - {r}"
-    using hLet.IH(2)[OF no_tails(2) inv(3) args_invar(2) rel_rgt(2) rel_state2] by blast
-
-  have "s = s2 on set stale - {r}" using ih1 fresh_not_in_stale eq_on_subset by blast
-  moreover have "s2 = s3 on set stale - {r}" using ih2 fresh_not_in_stale by auto
-  ultimately have s3_like_s: "s = s3 on set stale - {r}" by blast
+  have s2_like_s3: "s3 = s2 on set f_args \<union> set bs \<union> set keep - {r}"
+    using Un_Diff ih2(3) by auto
+  with s_like_s2 have s_like_s3: "s3 = s on set f_args \<union> set bs \<union> set keep - {r}"
+    by (simp add: eq_on_def)
 
   show ?case
-    apply (simp add: Let_def)
-    apply (repeat \<open>rule exI\<close>; repeat \<open>rule conjI\<close>)
-    apply (rule tbig_step_t.tSeq)
-    using ih1 ih2 s3_like_s by auto
+    unfolding to_imp_tc.simps Let_def
+    using ih1 ih2 s_like_s3 by blast
 next
   case (hLetBound n)
   show ?case
   proof (repeat \<open>rule exI\<close>; repeat \<open>rule conjI\<close>)
     from hLetBound_case hLetBound have "v = vs_b ! n" "n < length vs_b" by auto
     then have "aval (A (V (bs ! n))) s = v" using hLetBound unfolding relate_exec_state_def by auto
-    then show "f_c \<turnstile> (to_imp_tc f_args crgt bs r stale (hLetBound n), s) \<Rightarrow>\<^bsup>Suc (Suc 0)\<^esup> s(r := v)"
+    then show "f_c \<turnstile> (to_imp_tc f_args crgt bs r keep (hLetBound n), s) \<Rightarrow>\<^bsup>Suc (Suc 0)\<^esup> s(r := v)"
       by (metis tbig_step_t.tAssign to_imp_tc.simps(3))
   qed (simp_all add: eq_on_def)
 next
@@ -252,7 +388,7 @@ next
   proof (repeat \<open>rule exI\<close>; repeat \<open>rule conjI\<close>)
     from hArg_case hArg have "v = vs_arg ! n" "n < length vs_arg" by auto
     then have "aval (A (V (f_args ! n))) s = v" using hArg unfolding relate_exec_state_def by auto
-    then show "f_c \<turnstile> (to_imp_tc f_args crgt bs r stale (hArg n), s) \<Rightarrow>\<^bsup>Suc (Suc 0)\<^esup> s(r := v)"
+    then show "f_c \<turnstile> (to_imp_tc f_args crgt bs r keep (hArg n), s) \<Rightarrow>\<^bsup>Suc (Suc 0)\<^esup> s(r := v)"
       by (metis tbig_step_t.tAssign to_imp_tc.simps(4))
   qed (simp_all add: eq_on_def)
 next
@@ -260,111 +396,227 @@ next
   show ?case
   proof (repeat \<open>rule exI\<close>; repeat \<open>rule conjI\<close>)
     have "aval (A (N n)) s = v" using hNumber unfolding relate_exec_state_def by auto
-    then show "f_c \<turnstile> (to_imp_tc f_args crgt bs r stale (hNumber n), s) \<Rightarrow>\<^bsup>Suc (Suc 0)\<^esup> s(r := v)"
+    then show "f_c \<turnstile> (to_imp_tc f_args crgt bs r keep (hNumber n), s) \<Rightarrow>\<^bsup>Suc (Suc 0)\<^esup> s(r := v)"
       by (metis tbig_step_t.tAssign to_imp_tc.simps(5))
   qed (simp_all add: eq_on_def)
 next
   case (hIf t1 t2 t3)
 
-  let ?r1 = "fresh' stale ''If.x''"
+  let ?r1 = "fresh' (stale_registers f_args crgt bs keep (IF t1\<noteq>0 THEN t2 ELSE t3)) ''If.x''"
 
   have no_tails: "\<not> HOL_TCN_Timing.tails t1" "\<not> HOL_TCN_Timing.tails t2" "\<not> HOL_TCN_Timing.tails t3" using hIf by simp_all
-
-  have args_invar: "compiler_args_invar f_args crgt bs stale t1" "compiler_args_invar f_args crgt bs stale t2" "compiler_args_invar f_args crgt bs stale t3"
-    using hIf unfolding compiler_args_invar_def reserved_regs_def split_beta by auto
+  then have "invar t1" "invar t2" "invar t3" by simp_all
+  then have args_invar:
+      "compiler_args_invar crgt f_args bs keep t1"
+      "compiler_args_invar crgt f_args bs keep t2"
+      "compiler_args_invar crgt f_args bs keep t3"
+    using hIf.prems compiler_args_invar_subset[where t = t1 and t' = "IF t1\<noteq>0 THEN t2 ELSE t3"] apply simp
+    using hIf.prems compiler_args_invar_subset[where t = t2 and t' = "IF t1\<noteq>0 THEN t2 ELSE t3"] apply fastforce
+    using hIf.prems compiler_args_invar_subset[where t = t3 and t' = "IF t1\<noteq>0 THEN t2 ELSE t3"] apply fastforce (* TODO ? *)
+    done
 
   have rel_rgt: "relate_rgt_correctness frgt crgt (calls_r t1)" "relate_rgt_correctness frgt crgt (calls_r t2)" "relate_rgt_correctness frgt crgt (calls_r t3)"
-    using hIf unfolding relate_rgt_correctness_def by auto
+    using hIf unfolding relate_rgt_correctness_def by simp_all
 
   have rel_state1: "relate_exec_state f_args bs vs_arg vs_b s" using hIf by blast
-
-  have res_reg_subset: "set f_args \<subseteq> set stale - {?r1}" "set bs \<subseteq> set stale - {?r1}"
-    using hIf.prems(3) fresh_not_in_stale unfolding compiler_args_invar_def reserved_regs_def by simp_all
 
   show ?case
   proof (cases rule: hIf_case[OF hIf.prems(2)])
     case (1 z1 v1 z2)
 
-    obtain z1_c s2 where
-      ih1: "f_c \<turnstile> (to_imp_tc f_args crgt bs ?r1 stale t1, s) \<Rightarrow>\<^bsup>z1_c\<^esup>  s2" "s2 ?r1 = v1" "s = s2 on set stale - {?r1}"
-      using no_tails 1 args_invar rel_rgt rel_state1 hIf by metis
+    obtain z1_c s2 where ih1:
+        "f_c \<turnstile> (to_imp_tc f_args crgt bs ?r1 keep t1, s) \<Rightarrow>\<^bsup>z1_c\<^esup> s2"
+        "s2 ?r1 = v1" "s2 = s on set f_args \<union> set bs \<union> set keep - {?r1}"
+      using hIf.IH(1) no_tails(1) 1 args_invar(1) rel_rgt(1) rel_state1 by blast
 
-    have rel_state2: "relate_exec_state f_args bs vs_arg vs_b s2"
-      using hIf ih1 unfolding relate_exec_state_def apply simp
-      unfolding map_eq_on_subset_eq[OF res_reg_subset(1)] map_eq_on_subset_eq[OF res_reg_subset(2)] by blast
+    have s_like_s2: "s2 = s on set f_args \<union> set bs \<union> set keep" (* TODO *)
+      by (smt (verit) DiffI Un_iff eq_on_def fresh_not_in_stale ih1(3) set_append singletonD stale_registers_def)
+    then have rel_state2: "relate_exec_state f_args bs vs_arg vs_b s2"
+      using hIf.prems(5) unfolding relate_exec_state_def using ih1 by fastforce
 
-    obtain z2_c s3 where
-      ih2: "f_c \<turnstile> (to_imp_tc f_args crgt bs r stale t2, s2) \<Rightarrow>\<^bsup>z2_c\<^esup>  s3" "s3 r = v" "s2 = s3 on set stale - {r}"
-      using no_tails 1 args_invar rel_rgt rel_state2 hIf by metis
-
-    have "s = s2 on set stale - {r}" using ih1 fresh_not_in_stale eq_on_subset by blast
-    moreover have "s2 = s3 on set stale - {r}" using ih2 fresh_not_in_stale by auto
-    ultimately have s3_like_s: "s = s3 on set stale - {r}" by blast
-
-    show ?thesis apply (simp add: Let_def) apply (repeat \<open>rule exI\<close>; repeat \<open>rule conjI\<close>)
-        apply (rule tbig_step_t.tSeq) using ih1 apply blast apply (rule tbig_step_t.tIfTrue) using ih1 1 apply simp using ih2 apply simp apply simp apply simp
-        using ih2 apply simp using s3_like_s by auto
+    obtain z2_c s3 where ih2:
+        "f_c \<turnstile> (to_imp_tc f_args crgt bs r keep t2, s2) \<Rightarrow>\<^bsup>z2_c\<^esup>  s3" "s3 r = v"
+        "s3 = s2 on set f_args \<union> set bs \<union> set keep - {r}"
+      using hIf.IH(2) no_tails(2) 1 args_invar(2) rel_rgt(2) rel_state2 by blast
+  
+    have s2_like_s3: "s3 = s2 on set f_args \<union> set bs \<union> set keep - {r}"
+      using Un_Diff ih2(3) by auto
+    with s_like_s2 have s_like_s3: "s3 = s on set f_args \<union> set bs \<union> set keep - {r}"
+      by (simp add: eq_on_def)
+  
+    show ?thesis
+      unfolding to_imp_tc.simps Let_def
+      using ih1 ih2 s_like_s3 1 by blast
   next
     case (2 z1 z2)
 
-    obtain z1_c s2 where
-      ih1: "f_c \<turnstile> (to_imp_tc f_args crgt bs ?r1 stale t1, s) \<Rightarrow>\<^bsup>z1_c\<^esup>  s2" "s2 ?r1 = 0" "s = s2 on set stale - {?r1}"
-      using no_tails 2 args_invar rel_rgt rel_state1 hIf by metis
+    obtain z1_c s2 where ih1:
+        "f_c \<turnstile> (to_imp_tc f_args crgt bs ?r1 keep t1, s) \<Rightarrow>\<^bsup>z1_c\<^esup> s2"
+        "s2 ?r1 = 0" "s2 = s on set f_args \<union> set bs \<union> set keep - {?r1}"
+      using hIf.IH(1) no_tails(1) 2(2) args_invar(1) rel_rgt(1) rel_state1 by metis
 
-    have rel_state2: "relate_exec_state f_args bs vs_arg vs_b s2"
-      using hIf ih1 unfolding relate_exec_state_def apply simp
-      unfolding map_eq_on_subset_eq[OF res_reg_subset(1)] map_eq_on_subset_eq[OF res_reg_subset(2)] by blast
+    have s_like_s2: "s2 = s on set f_args \<union> set bs \<union> set keep" (* TODO *)
+      by (smt (verit) DiffI Un_iff eq_on_def fresh_not_in_stale ih1(3) set_append singletonD stale_registers_def)
+    then have rel_state3: "relate_exec_state f_args bs vs_arg vs_b s2"
+      using hIf.prems(5) unfolding relate_exec_state_def using ih1 by fastforce
 
-    obtain z2_c s3 where
-      ih2: "f_c \<turnstile> (to_imp_tc f_args crgt bs r stale t3, s2) \<Rightarrow>\<^bsup>z2_c\<^esup>  s3" "s3 r = v" "s2 = s3 on set stale - {r}"
-      using no_tails 2 args_invar rel_rgt rel_state2 hIf by metis
-
-    have "s = s2 on set stale - {r}" using ih1 fresh_not_in_stale eq_on_subset by blast
-    moreover have "s2 = s3 on set stale - {r}" using ih2 fresh_not_in_stale by auto
-    ultimately have s3_like_s: "s = s3 on set stale - {r}" by blast
-
-    show ?thesis apply (simp add: Let_def) apply (repeat \<open>rule exI\<close>; repeat \<open>rule conjI\<close>)
-        apply (rule tbig_step_t.tSeq) using ih1 apply blast apply (rule tbig_step_t.tIfFalse) using ih1 2 apply simp using ih2 apply simp apply simp apply simp
-        using ih2 apply simp using s3_like_s by auto
+    obtain z2_c s3 where ih3:
+        "f_c \<turnstile> (to_imp_tc f_args crgt bs r keep t3, s2) \<Rightarrow>\<^bsup>z2_c\<^esup>  s3" "s3 r = v"
+        "s3 = s2 on set f_args \<union> set bs \<union> set keep - {r}"
+      using hIf.IH(3) no_tails(3) 2 args_invar(3) rel_rgt(3) rel_state3 by blast
+  
+    have s2_like_s3: "s3 = s2 on set f_args \<union> set bs \<union> set keep - {r}"
+      using Un_Diff ih3(3) by auto
+    with s_like_s2 have s_like_s3: "s3 = s on set f_args \<union> set bs \<union> set keep - {r}"
+      by (simp add: eq_on_def)
+  
+    show ?thesis
+      unfolding to_imp_tc.simps Let_def
+      using ih1 ih3 s_like_s3 2 by blast
   qed
 next
   case (hCall gr ts)
 
-  obtain g T_g zs vs where
-          z: "z = sum_list zs + T_g vs"
-      and gr: "(g, T_g) = frgt gr"
+  let ?g = "f_from_frgt frgt gr"
+  let ?T_g = "T_f_from_frgt frgt gr"
+
+  obtain zs vs where
+          z: "z = sum_list zs + ?T_g vs"
       and lengths: "length zs = length ts" "length vs = length ts"
       and args_bigstep: "\<forall>i<length ts. (f, frgt) \<turnstile> (ts ! i, vs_b, vs_arg) \<Rightarrow>\<^bsup>zs ! i\<^esup> vs ! i"
-      and gvs: "g vs = v"
-    using hCall_case hCall by blast
+      and gvs: "?g vs = v"
+    using hCall_case hCall split_from_frgt by auto
 
 
-  let ?xs = "make_n_fresh stale ''Call.x.'' (length ts)"
-  let ?c1_gen = "\<lambda>crgt st. t_seqs' (map (\<lambda>i. to_imp_tc f_args crgt bs (?xs ! i) st (ts ! i)) [0..<length ts])"
-  let ?crgt_gen = "crgt(gr := (take (length ts) (args_from_crgt crgt gr), com_from_crgt crgt gr, ret_from_crgt crgt gr))"
-  let ?c1 = "?c1_gen crgt (?xs @ stale)"
-  let ?c2 = "t_seqs' (map (\<lambda>i. (args_from_crgt crgt gr ! i) ::= A (V (?xs ! i))) [0..<length ts])"
-  let ?c3 = "CALL com_from_crgt crgt gr RETURN ret_from_crgt crgt gr :: tcom"
+  (* part 1: computing the arguments *)
+
+  let ?xs = "make_n_fresh (stale_registers f_args crgt bs keep (hCall gr ts)) ''Call.x.'' (length ts)"
+  let ?c1 = "t_seqs' (generate (\<lambda>i. to_imp_tc f_args crgt bs (?xs ! i) (?xs @ keep) (ts ! i)) (length ts))"
+
+  obtain z1 s2 where exec_c1: "f_c \<turnstile> (?c1, s)\<Rightarrow>\<^bsup>z1\<^esup> s2" "lookups ?xs s2 = vs"
+      "s2 r = v" "s2 = s on set f_args \<union> set bs \<union> set (?xs @ keep) - set ?xs"
+    sorry (* TODO ! *)
+
+
+  (* part 2: copying from temporaries to argument registers *)
+
+  let ?c2 = "t_seqs' (generate (\<lambda>i. (args_from_crgt crgt gr ! i) ::= A (V (?xs ! i))) (length ts))"
+  let ?z2 = "Suc (2 * length ts)"
+
+  have "set (args_from_crgt crgt gr) \<subseteq> set (stale_registers f_args crgt bs keep (hCall gr ts))"
+    unfolding stale_registers_def call_registers_def by fastforce
+  then have dj: "set ?xs \<inter> set (args_from_crgt crgt gr) = {}"
+    using make_n_fresh_not_in_stale by blast
+  moreover have "distinct (args_from_crgt crgt gr)"
+    using hCall.prems unfolding compiler_args_invar_def by simp
+  moreover have "length ?xs = length ts"
+    unfolding make_n_fresh_def generate_def by simp
+  moreover have "length (args_from_crgt crgt gr) = length ts"
+    using hCall.prems unfolding compiler_args_invar_def by simp
+
+  ultimately obtain s3 where exec_c2: "f_c \<turnstile> (?c2, s2) \<Rightarrow>\<^bsup>?z2\<^esup> s3"
+       "lookup_args crgt gr s3 = lookups ?xs s2" "s3 = s2 on - set (args_from_crgt crgt gr)"
+    using copy_list_sem' by blast
+
+
+  (* part 3: calling g *)
+  
+  let ?gcom = "com_from_crgt crgt gr" and ?gret = "ret_from_crgt crgt gr" and ?gv = "f_from_frgt frgt gr (lookup_args crgt gr s3)"
+  let ?c3 = "CALL ?gcom RETURN ?gret :: tcom"
+  let ?s4 = "s3(?gret := ?gv)"
+
+  have "terminates_with_res_IMP ?gcom s3 ?gret ?gv" using hCall.prems unfolding relate_rgt_correctness_def by simp
+  then obtain z3 s4' where "(?gcom, s3) \<Rightarrow>\<^bsup>z3\<^esup> s4'" "s4' ?gret = ?gv"
+    unfolding terminates_with_res_IMP_def terminates_with_res_pred_time_IMP_def terminates_with_pred_time_IMP_def by blast
+  then have exec_c3: "f_c \<turnstile> (?c3, s3) \<Rightarrow>\<^bsup>z3\<^esup> ?s4" using tbig_step_t.tCall by metis
+
+  have "f_from_frgt frgt gr = ?g" using split_from_frgt by simp
+  then have vfrom: "?gv = v" using exec_c1(2) exec_c2(2) gvs by simp
+
+
+  (* part 4: copying to r *)
+
   let ?c4 = "r ::= A (V (ret_from_crgt crgt gr)) :: tcom"
 
-  (* let ?compiler_args_invar_weak = "\<lambda>f_args crgt bs stale t. *)
+  let ?s5 = "?s4(r := aval (A (V ?gret)) ?s4)"
+  obtain z4 where exec_c4: "f_c \<turnstile> (?c4, ?s4) \<Rightarrow>\<^bsup>z4\<^esup> ?s5" by blast
+  then have s5: "?s5 = ?s4(r := v)" using vfrom exec_c3 by simp
+
+
+  (* putting it together *)
+
+  show ?case unfolding to_imp_tc.simps Let_def split_beta
+  proof (repeat \<open>rule exI\<close>; repeat \<open>rule conjI\<close>)
+    show "f_c \<turnstile> (?c1;; ?c2;; ?c3;; ?c4, s) \<Rightarrow>\<^bsup>z1 + ?z2 + z3 + z4\<^esup> ?s5"
+    apply (repeat \<open>rule tbig_step_t.tSeq\<close>)
+      using exec_c1 exec_c2 exec_c3 exec_c4 using tbig_step_t.tSeq by auto
+  next
+    show "?s5 r = v" using s5 by simp
+  next
+    have "set f_args \<union> set bs \<union> set (?xs @ keep) - set ?xs = set f_args \<union> set bs \<union> set keep"
+      using make_n_fresh_not_in_stale unfolding stale_registers_def by fastforce
+    then have *: "s2 = s on set f_args \<union> set bs \<union> set keep - {r}"
+      using exec_c1 by blast
+
+    have "set f_args \<union> set bs \<union> set keep \<inter>\<^sub>\<emptyset> set (args_from_crgt crgt gr)"
+      using hCall.prems(3) unfolding compiler_args_invar_def call_registers_def by auto
+    then have **: "s3 = s2 on set f_args \<union> set bs \<union> set keep - {r}"
+      using hCall.prems(3) exec_c2 unfolding compiler_args_invar_def by auto
+
+    have "ret_from_crgt crgt gr \<notin> set f_args \<union> set bs \<union> set keep"
+      using hCall.prems(3) unfolding compiler_args_invar_def call_registers_def by auto
+    then have ***: "?s5 = s3 on set f_args \<union> set bs \<union> set keep - {r}" by auto
+
+    show "?s5 = s on set f_args \<union> set bs \<union> set keep - {r}"
+      using * ** *** by fastforce
+  qed
+
+
+
+
+  have "s2 = s on set keep" using s2 .
+  have "set keep \<subseteq> - set (args_from_crgt crgt gr)"
+    using hCall.prems unfolding compiler_args_invar_def reserved_regs_def 
+(* not equal on all of keep! have to fix lemma *) sorry
+  have "s3 = s2 on set keep" using s3 using hCall.prems unfolding compiler_args_invar_def reserved_regs_def 
+  have "s = ?s5 on set keep - {r}" using s2 s3 s4 s5 apply simp
+  
+
+  thm hCall_case[OF hCall.prems(2)]
+  have ?case
+  apply (simp only: to_imp_tc.simps Let_def split_beta mapi_map cc_call_helper[symmetric])
+  proof (repeat \<open>rule exI\<close>; repeat \<open>rule conjI\<close>)
+    apply (subst sym[OF cc_call_helper]) sorry
+
+
+
+(* end *)
+
+
+
+  let ?c1_gen = "\<lambda>crgt st. t_seqs' (map (\<lambda>i. to_imp_tc f_args crgt bs (?xs ! i) st (ts ! i)) [0..<length ts])"
+  let ?crgt_gen = "crgt(gr := (take (length ts) (args_from_crgt crgt gr), com_from_crgt crgt gr, ret_from_crgt crgt gr))"
+  let ?c1 = "?c1_gen crgt (?xs @ keep)"
+  let ?c2 = "t_seqs' (map (\<lambda>i. (args_from_crgt crgt gr ! i) ::= A (V (?xs ! i))) [0..<length ts])"
+
+  (* let ?compiler_args_invar_weak = "\<lambda>f_args crgt bs keep t. *)
         (* HOL_TCN_Timing.invar t *)
-        (* \<and> set (reserved_regs f_args crgt bs t) \<subseteq> set stale *)
+        (* \<and> set (reserved_regs f_args crgt bs t) \<subseteq> set keep *)
         (* \<and> distinct f_args *)
         (* \<and> (\<forall>(g,_) \<in> set (calls t). distinct (args_from_crgt crgt g))" *)
   (* from hCall(4) *)
-  (* have args_invar': "?compiler_args_invar_weak f_args crgt bs stale (hCall gr ts)" *)
+  (* have args_invar': "?compiler_args_invar_weak f_args crgt bs keep (hCall gr ts)" *)
     (* unfolding compiler_args_invar_def by simp *)
-  have "\<exists>z1 s2. f_c \<turnstile> (?c1_gen crgt st,s) \<Rightarrow>\<^bsup>z1\<^esup> s2 \<and> lookups ?xs s2 = vs \<and> s = s2 on set stale"
-    if "set (?xs @ stale) \<subseteq> set st" "length ts = length (args_from_crgt crgt gr)" for st
+  have "\<exists>z1 s2. f_c \<turnstile> (?c1_gen crgt st,s) \<Rightarrow>\<^bsup>z1\<^esup> s2 \<and> lookups ?xs s2 = vs \<and> s = s2 on set keep"
+    if "set (?xs @ keep) \<subseteq> set st" "length ts = length (args_from_crgt crgt gr)" for st
   using hCall(1,2,4,5,6) that args_bigstep proof (induction ts zs vs arbitrary: z v st crgt gr rule: snoc_list_induct3)
     case Nil then show ?case unfolding make_n_fresh_def by auto
   next
     case (snoc ts_arg t_arg zs0 z0 vs0 v0)
 
-    let ?xs = "make_n_fresh stale ''Call.x.'' (length ts_arg)"
-    let ?xs' = "make_n_fresh stale ''Call.x.'' (length (ts_arg @ [t_arg]))"
-    let ?x = "make_nth_fresh stale ''Call.x.'' (length ts_arg)"
+    let ?xs = "make_n_fresh keep ''Call.x.'' (length ts_arg)"
+    let ?xs' = "make_n_fresh keep ''Call.x.'' (length (ts_arg @ [t_arg]))"
+    let ?x = "make_nth_fresh keep ''Call.x.'' (length ts_arg)"
     have xs': "?xs' = ?xs @ [?x]" unfolding make_n_fresh_def using nth_map_upt by simp
     have x: "?xs' ! length ts_arg = ?x" unfolding xs' unfolding make_n_fresh_def by (subst nth_append) simp
 
@@ -377,7 +629,7 @@ next
       (* apply (induction ts_arg) apply auto *)
     thm snoc
     thm snoc.IH
-    have "\<exists>z1 s2. f_c \<turnstile> (?c1, s) \<Rightarrow>\<^bsup>z1\<^esup>  s2 \<and> lookups ?xs s2 = vs0 \<and> s = s2 on set stale"
+    have "\<exists>z1 s2. f_c \<turnstile> (?c1, s) \<Rightarrow>\<^bsup>z1\<^esup>  s2 \<and> lookups ?xs s2 = vs0 \<and> s = s2 on set keep"
       apply (rule snoc.IH[where gr = gr]) (* ?gr' *)
       subgoal using snoc.prems(1) by simp
       subgoal using snoc.prems(2) by simp
@@ -397,7 +649,7 @@ next
         sorry
       subgoal sorry
       done
-    then obtain z1 s2 where ih1: "f_c \<turnstile> (?c1, s) \<Rightarrow>\<^bsup>z1\<^esup> s2" "lookups ?xs s2 = vs0" "s = s2 on set stale"
+    then obtain z1 s2 where ih1: "f_c \<turnstile> (?c1, s) \<Rightarrow>\<^bsup>z1\<^esup> s2" "lookups ?xs s2 = vs0" "s = s2 on set keep"
       by blast
 
 
@@ -431,10 +683,9 @@ next
       using snoc.prems unfolding relate_rgt_correctness_def by auto
 
     have exec_t_arg: "(f, frgt) \<turnstile> (t_arg, vs_b, vs_arg) \<Rightarrow>\<^bsup>z0\<^esup> v0" using snoc.prems
-      by (metis length_append_singleton lessI nth_append_length
-          snoc.hyps(1,2))
+      by (metis length_append_singleton lessI nth_append_length snoc.hyps(1,2))
 
-    have "set f_args \<subseteq> set stale" "set bs \<subseteq> set stale"
+    have "set f_args \<subseteq> set keep" "set bs \<subseteq> set keep"
       using snoc.prems unfolding compiler_args_invar_def reserved_regs_def by simp_all
     then have rel_state: "relate_exec_state f_args bs vs_arg vs_b s2" using snoc.prems(5) ih1
       unfolding relate_exec_state_def using eq_on_subset by fastforce
@@ -449,13 +700,13 @@ next
       have "?x \<notin> set ?xs"
         apply (subst sym[OF none_equal_not_in])
         using make_n_fresh_def inj_on_contraD[OF inj_make_nth_fresh] by simp (* this should not be so hard... *)
-      then have "set ?xs \<subseteq> set (?xs' @ stale) - {?x}" using xs' fresh_not_in_stale unfolding make_nth_fresh_def by simp
+      then have "set ?xs \<subseteq> set (?xs' @ keep) - {?x}" using xs' fresh_not_in_keep unfolding make_nth_fresh_def by simp
       also have "... \<subseteq> set st - {?x}" using snoc.prems by blast
       finally show "lookups ?xs' s3 = vs0 @ [v0]"
         using xs' ih1 texec_t_arg by fastforce
     next
-      show "s = s3 on set stale"
-        using ih1 texec_t_arg fresh_not_in_stale make_nth_fresh_def snoc.prems(6) by fastforce
+      show "s = s3 on set keep"
+        using ih1 texec_t_arg fresh_not_in_keep make_nth_fresh_def snoc.prems(6) by fastforce
     next
       have 1: "map (\<lambda>i. to_imp_tc f_args crgt bs (?xs' ! i) st ((ts_arg @ [t_arg]) ! i)) [0..<length (ts_arg @ [t_arg])]
         = map (\<lambda>i. to_imp_tc f_args crgt bs (?xs ! i) st (ts_arg ! i)) [0..<length ts_arg] @ [?c2]"
@@ -472,7 +723,7 @@ next
 
   moreover have lll: "length ts = length (args_from_crgt crgt gr)"
     using hCall.prems unfolding compiler_args_invar_def by simp
-  ultimately obtain z1 s2 where exec_c1: "f_c \<turnstile> (?c1,s) \<Rightarrow>\<^bsup>z1\<^esup> s2" and "lookups ?xs s2 = vs" and s2: "s = s2 on set stale"
+  ultimately obtain z1 s2 where exec_c1: "f_c \<turnstile> (?c1,s) \<Rightarrow>\<^bsup>z1\<^esup> s2" and "lookups ?xs s2 = vs" and s2: "s = s2 on set keep"
     using hCall.prems unfolding compiler_args_invar_def by blast
 
 
@@ -481,19 +732,19 @@ next
   have lll2: "length ?xs = length (args_from_crgt crgt gr)"
     using lll unfolding make_n_fresh_def by simp
 
-  have "set (args_from_crgt crgt gr) \<subseteq> set stale"
+  have "set (args_from_crgt crgt gr) \<subseteq> set keep"
     using hCall.prems unfolding compiler_args_invar_def reserved_regs_def by simp
   then have ddd: "distinct (?xs @ args_from_crgt crgt gr)"
-    apply simp using hCall.prems make_n_fresh_not_in_stale unfolding compiler_args_invar_def apply simp
+    apply simp using hCall.prems make_n_fresh_not_in_keep unfolding compiler_args_invar_def apply simp
     apply (rule Int_emptyI) by blast
 
   thm copy_list_sem
   thm copy_list_sem[where s = s2 and f = f_c and xs = ?xs and ys = "args_from_crgt crgt gr", OF lll2 ddd]
 
   obtain s3 where "f_c \<turnstile> (t_seqs'
-               (map (\<lambda>i. (args_from_crgt crgt gr ! i) ::= A (V (make_n_fresh stale ''Call.x.'' (length ts) ! i)))
-                 [0..<length (make_n_fresh stale ''Call.x.'' (length ts))]),
-              s2) \<Rightarrow>\<^bsup>Suc (2 * length (make_n_fresh stale ''Call.x.'' (length ts)))\<^esup>  s3"
+               (map (\<lambda>i. (args_from_crgt crgt gr ! i) ::= A (V (make_n_fresh keep ''Call.x.'' (length ts) ! i)))
+                 [0..<length (make_n_fresh keep ''Call.x.'' (length ts))]),
+              s2) \<Rightarrow>\<^bsup>Suc (2 * length (make_n_fresh keep ''Call.x.'' (length ts)))\<^esup>  s3"
       "lookups ?xs s2 = lookup_args crgt gr s3 " and s3: "s2 = s3 on - set (args_from_crgt crgt gr)"
     using copy_list_sem[OF lll2 ddd] by blast
   then obtain z2 where exec_c2: "f_c \<turnstile> (?c2, s2) \<Rightarrow>\<^bsup>z2\<^esup> s3"
@@ -528,12 +779,12 @@ next
 
   have "?s5 r = v" using s5 by simp
 
-  have "s = s2 on set stale" using s2 .
-  have "set stale \<subseteq> - set (args_from_crgt crgt gr)"
+  have "s = s2 on set keep" using s2 .
+  have "set keep \<subseteq> - set (args_from_crgt crgt gr)"
     using hCall.prems unfolding compiler_args_invar_def reserved_regs_def 
-(* not equal on all of stale! have to fix lemma *) sorry
-  have "s2 = s3 on set stale" using s3 using hCall.prems unfolding compiler_args_invar_def reserved_regs_def 
-  have "s = ?s5 on set stale - {r}" using s2 s3 s4 s5 apply simp
+(* not equal on all of keep! have to fix lemma *) sorry
+  have "s2 = s3 on set keep" using s3 using hCall.prems unfolding compiler_args_invar_def reserved_regs_def 
+  have "s = ?s5 on set keep - {r}" using s2 s3 s4 s5 apply simp
   
 
   thm hCall_case[OF hCall.prems(2)]
@@ -551,13 +802,13 @@ next
 
   have calls_subset: "set (calls (ts ! i)) \<subseteq> set (calls (hCall gr ts))" if "i < length ts" for i using hCall tsi_in_ts that by fastforce
 
-  have args_invar: "compiler_args_invar f_args crgt bs stale (ts ! i)" if "i < length ts" for i
+  have args_invar: "compiler_args_invar f_args crgt bs keep (ts ! i)" if "i < length ts" for i
   unfolding compiler_args_invar_def proof (repeat \<open>rule conjI\<close>)
     show "HOL_TCN_Timing.invar (ts ! i)" using no_tails_invar no_tails that by blast
   next
     have "set (reserved_regs f_args crgt bs (ts ! i)) \<subseteq> set (reserved_regs f_args crgt bs (hCall gr ts))"
       unfolding reserved_regs_def using calls_subset that by fastforce
-    then show "set (reserved_regs f_args crgt bs (ts ! i)) \<subseteq> set stale"
+    then show "set (reserved_regs f_args crgt bs (ts ! i)) \<subseteq> set keep"
       using hCall unfolding compiler_args_invar_def by auto
   next
     show "distinct f_args" using hCall compiler_args_invar_def by simp
@@ -569,7 +820,7 @@ next
   
 (* 
   have no_tails: "\<not> HOL_TCN_Timing.tails (ts ! i)"
-    and args_invar: "compiler_args_invar f_args crgt bs stale (ts ! i)"
+    and args_invar: "compiler_args_invar f_args crgt bs keep (ts ! i)"
     (* and "set (calls (ts ! i)) \<subseteq> set (calls (hCall gr ts))" *)
     if "i < length ts" for i
     (* using hCall tsi_in_ts that by auto *)
@@ -584,7 +835,7 @@ next
     
 
   have "set (calls (ts ! i)) \<subseteq> set (calls (hCall gr ts))" if "i < length ts" for i using hCall tsi_in_ts that by fastforce
-  then have args_invar: "compiler_args_invar f_args crgt bs stale (ts ! i)" if "i < length ts" for i
+  then have args_invar: "compiler_args_invar f_args crgt bs keep (ts ! i)" if "i < length ts" for i
     using hCall tsi_in_ts that unfolding compiler_args_invar_def reserved_regs_def apply simp
 
   show ?case
@@ -724,10 +975,10 @@ thm tto_end_non_tail tto_end_tail *)
 find_theorems "map fst"
 lemma
   assumes compiler_correct_nt_: True
-  fixes t_imp f_args crgt frgt bs r stale t vs_b vs_arg
-  defines "t_imp \<equiv> to_imp_tc f_args crgt bs r stale t"
+  fixes t_imp f_args crgt frgt bs r keep t vs_b vs_arg
+  defines "t_imp \<equiv> to_imp_tc f_args crgt bs r keep t"
   assumes "t_time \<equiv> time_to_tail frgt vs_b vs_arg t"
-  assumes "well_formed_comp f_args crgt bs stale t"
+  assumes "well_formed_comp f_args crgt bs keep t"
   assumes "well_encoded_comp f_args bs vs_arg vs_b s"
   (* assumes "called_correctness crgt frgt t" *)
   shows "\<exists>k Cs.
@@ -735,7 +986,7 @@ lemma
     \<and> length Cs = length t_time
     \<and> (\<forall>((C,s), (g,vs_arg_g)) \<in> set (zip Cs t_time).
           C = com_from_crgt crgt g \<and> vs_arg_g = lookup_args crgt g s)"
-using assms(2-4) proof (induction t arbitrary: t_imp t_time bs r stale vs_b s)
+using assms(2-4) proof (induction t arbitrary: t_imp t_time bs r keep vs_b s)
   case (hLet t1 t2)
   then show ?case sorry
 next
@@ -752,8 +1003,8 @@ next
   then show ?case sorry
 next
   case (hCall g ts)
-  let ?xs = "make_n_fresh (length ts) stale ''Call.x.''"
-  let ?cs1 = "mapi (\<lambda>i t. to_imp_tc f_args crgt bs (?xs ! i) (?xs @ stale) t) ts"
+  let ?xs = "make_n_fresh (length ts) keep ''Call.x.''"
+  let ?cs1 = "mapi (\<lambda>i t. to_imp_tc f_args crgt bs (?xs ! i) (?xs @ keep) t) ts"
   let ?cs2 = "mapi (\<lambda>i t. tAssign (args_from_crgt crgt g ! i) (A (V (?xs ! i)))) ts"
   let ?call = "tSeq (tCall (com_from_crgt crgt g) (ret_from_crgt crgt g)) (tAssign r (A (V (ret_from_crgt crgt g))))"
 
@@ -779,32 +1030,32 @@ qed
 
 lemma
   assumes compiler_correct_nt_: True
-  assumes "t_imp = to_imp_tc f_args crgt bs r stale t"
-  assumes "well_formed_comp f_args crgt bs stale t"
+  assumes "t_imp = to_imp_tc f_args crgt bs r keep t"
+  assumes "well_formed_comp f_args crgt bs keep t"
   assumes "well_encoded_comp f_args bs vs_arg vs_b s"
   assumes "called_correctness crgt frgt t"
   shows "\<exists>k z.
     ttime_to_tail s t_imp (k + z)
     \<and> k \<le> tstruct_k t_imp
     \<and> z \<le> tinterp_time frgt crgt (time_to_tail frgt vs_b vs_arg t)"
-using assms(2-5) proof (induction t arbitrary: t_imp bs r stale vs_b s)
+using assms(2-5) proof (induction t arbitrary: t_imp bs r keep vs_b s)
   case (hLet t1 t2)
   thm hLet.prems(1)[simplified]
   thm hLet.IH(1) hLet.IH(2)
 
   thm hLet.prems
 
-  let ?x_var = "fresh' stale ''Let.x''"
-  let ?t_imp1 = "to_imp_tc f_args crgt bs ?x_var stale t1"
+  let ?x_var = "fresh' keep ''Let.x''"
+  let ?t_imp1 = "to_imp_tc f_args crgt bs ?x_var keep t1"
 
-  have wf1: "well_formed_comp f_args crgt bs stale t1" using hLet.prems(2)
+  have wf1: "well_formed_comp f_args crgt bs keep t1" using hLet.prems(2)
     unfolding well_formed_comp_def using non_tail_tailrec apply auto apply (simp only: reserved_regs_def h_calls.simps map_append)
     by auto
   then obtain k1 z1 where k1z1:
       "ttime_to_tail s ?t_imp1 (k1 + z1)"
       "k1 \<le> tstruct_k ?t_imp1"
       "z1 \<le> tinterp_time frgt crgt (time_to_tail frgt vs_b vs_arg t1)"
-    using hLet.IH(1)[where t_imp = ?t_imp1 and s = s and bs = bs and vs_b = vs_b and r = ?x_var and stale = stale] hLet.prems
+    using hLet.IH(1)[where t_imp = ?t_imp1 and s = s and bs = bs and vs_b = vs_b and r = ?x_var and keep = keep] hLet.prems
     unfolding called_correctness_def by auto
 
   have ob1: "non_tail t1" using hLet unfolding well_formed_comp_def by simp
@@ -812,24 +1063,24 @@ using assms(2-5) proof (induction t arbitrary: t_imp bs r stale vs_b s)
   obtain f y1 s1
       where t1s1: "f \<turnstile> (?t_imp1,s) \<Rightarrow>\<^bsup>y1\<^esup> s1"
       and s1_xvar: "s1 ?x_var = eval_non_tail frgt vs_b vs_arg t1"
-      and s1: "s = s1 on (Set.remove ?x_var (set stale))"
+      and s1: "s = s1 on (Set.remove ?x_var (set keep))"
     using compiler_correct_nt[OF ob1 wf1 ob2, simplified] by blast
 
   have "tailrec t1" using well_formed_comp_def wf1 by blast
   then have inv: "invar ?t_imp1" using to_imp_invar by blast
   have y1: "y1 = k1 + z1" using ttime_non_tail[OF inv t1s1] sorry (* ttime_to_tail for non-tail MUST INVESTIGATE AND WRITE LEMMA *)
 
-  let ?t_imp2 = "to_imp_tc f_args crgt (?x_var # bs) r (?x_var # stale) t2"
+  let ?t_imp2 = "to_imp_tc f_args crgt (?x_var # bs) r (?x_var # keep) t2"
   have "tailrec t2" using hLet unfolding well_formed_comp_def by simp
 
-  have t2_1: "well_formed_comp f_args crgt (?x_var # bs) (?x_var # stale) t2"
+  have t2_1: "well_formed_comp f_args crgt (?x_var # bs) (?x_var # keep) t2"
     using hLet.prems(2) unfolding well_formed_comp_def apply auto sorry (* almost sub-term *)
-  have "set f_args \<subseteq> Set.remove ?x_var (set stale)" using fresh_not_in_stale
+  have "set f_args \<subseteq> Set.remove ?x_var (set keep)" using fresh_not_in_keep
     unfolding remove_def apply simp using hLet.prems(2) unfolding well_formed_comp_def reserved_regs_def by simp
   then have t2_2_1: "lookups f_args s1 = vs_arg"
     apply (subst lookups_eq_on[where s = s, symmetric])
     using s1 apply blast using hLet.prems(3) unfolding well_encoded_comp_def by blast
-  have "set bs \<subseteq> Set.remove ?x_var (set stale)" using fresh_not_in_stale
+  have "set bs \<subseteq> Set.remove ?x_var (set keep)" using fresh_not_in_keep
     unfolding remove_def apply simp using hLet.prems(2) unfolding well_formed_comp_def reserved_regs_def by simp
   then have t2_2_2: "lookups (?x_var # bs) s1 = eval_non_tail frgt vs_b vs_arg t1 # vs_b" apply auto
     using s1_xvar apply blast
@@ -843,7 +1094,7 @@ using assms(2-5) proof (induction t arbitrary: t_imp bs r stale vs_b s)
       "k2 \<le> tstruct_k ?t_imp2"
       "z2 \<le> tinterp_time frgt crgt (time_to_tail frgt (eval_non_tail frgt vs_b vs_arg t1 # vs_b) vs_arg t2)"
     using hLet.IH(2)[where t_imp = ?t_imp2 and r = r and s = s1 and bs = "?x_var # bs"
-      and vs_b = "eval_non_tail frgt vs_b vs_arg t1 # vs_b" and stale = "?x_var # stale", OF _ t2_1 t2_2 t2_3, simplified]
+      and vs_b = "eval_non_tail frgt vs_b vs_arg t1 # vs_b" and keep = "?x_var # keep", OF _ t2_1 t2_2 t2_3, simplified]
     by blast
 
   from t1s1 k2z2
